\section{Introduction to Astrodynamics}

\subsection{2-body Problem}
\begin{equation}
  \vec{\ddot{r}} = -\frac{G(M+m)}{r^3}\vec{r}
\end{equation}
Using $\mu = GM$,
\begin{equation}
  \vec{\ddot{r}} + \frac{\mu}{r^3}\vec{r} = 0
\end{equation}

\subsection{Elliptic Orbit Equations}
\begin{equation}
  b=a\sqrt{1-e^2}
\end{equation}
\begin{equation}
  p=b^2/a = a(1-e^2)
\end{equation}
\begin{equation}
  h=\sqrt{\mu p}
\end{equation}
\begin{equation}
  \epsilon=\frac{v^2}{2}-\frac{GM}{r}=-\frac{\mu}{2a}
\end{equation}

\subsection{Motion of a Satellite in Orbit}
\begin{equation}
  r = \frac{h^2/\mu}{1+E/\mu\cos(\nu)} = \frac{p}{1+e\cos(\nu)}
\end{equation}
where $p=b^2/a$ is the semi-latus rectum.

\subsection{Vis-Viva Equation}
Using Eq 1.6 and $h=r_pv_p=r_av_a$,
\begin{equation}
  \frac{1}{2}v_a^2=GM \frac{r_p}{r_a(r_p+r_a)}
\end{equation}
Therefore,
\begin{equation}
  v^2 = gM(\frac{2}{r}-\frac{1}{a})
\end{equation}

\subsection{Kepler's Equation}
\begin{equation}
  x=r\cos(\nu) = a(\cos(E)-e) \qquad y=r\sin(\nu) = a\sqrt{1-e^2}\sin(E)
\end{equation}
Using Eq. 1.5,
\begin{equation}
  E(t) - e\sin(E(t))=n(t-t_p) \longrightarrow M(t) = M_0 + n(t-t_p)
\end{equation}
where $n=\sqrt{\frac{\mu}{a^3}}$
\begin{equation}
  T=\frac{2\pi}{n}
\end{equation}
\textbf{In Orbital Elements}
\begin{equation}
  \vec{r} = \begin{pmatrix}
       a(\cos(E)-e)\\
       a\sqrt{1-e^2}\sin(E)\\
       0
       \end{pmatrix} \qquad
  \vec{v} = \frac{an}{1-e\cos(E)}\begin{pmatrix}
       -\sin(E)\\
       a\sqrt{1-e^2}\cos(E)\\
       0
       \end{pmatrix}
\end{equation}

\subsection{Orbital Perturbations}

\begin{equation}
  \frac{d\epsilon}{dt} = \vec{v}\cdot\vec{a_p} = \frac{\mu}{2a^2}\frac{da}{dt}
\end{equation}
\textbf{Atmospheric Drag}
\begin{equation}
  \vec{F_d} = -\frac{1}{2}C_dA\rho v^2\frac{\vec{v}}{v} \qquad \vec{a_p} = -\frac{C_dA}{2m}\rho v\vec{v}
\end{equation}
\begin{equation}
  \therefore \frac{da}{dt}=-\rho\sqrt{\mu a}\frac{C_dA}{m}
\end{equation}
\textbf{J2 Perturbation}
\begin{equation}
  \frac{d\Omega}{dt}=-\frac{3nJ_2R_e^2}{2a^2(1-e^2)^2}\cos(i)
\end{equation}
\begin{equation}
  \frac{d\omega}{dt}=\frac{2nJ_2R_e^2}{2a^2(1-e^2)^2}\left(\frac{5}{2}\sin^2(i)-2\right)
\end{equation}
where $J_2=0.001082$
